ROOT
@@ -1,11 +1,16 @@
 chapter AFP
 
 session "Isabelle_Lex-Yacc" (AFP) = HOL +
-  options [timeout = 600]
+  options [timeout = 1200]
+  directories
+    "C11"
   theories [document = false]
     Examples
+    "C11/C11_Tests"
+    "C11/AntiqProbe"
+    "C11/C11_Manual"
   theories
-    Manual 
+    Manual
   document_files
     "root.tex"
     "root.bib"
